src/DirSep.v
@@ -222,5 +222,27 @@ Proof.
   eapply dir2flatmem_find_subtree_ptsto; eauto.
 Qed.
 
+Lemma dir2flatmem_update_delete : forall tree basenum basedents base name,
+  tree_names_distinct tree ->
+  find_subtree base tree = Some (TreeDir basenum basedents) ->
+  dir2flatmem [] (update_subtree base (TreeDir basenum (delete_from_list name basedents)) tree) =
+  mem_except (dir2flatmem [] tree) (base++[name]).
+Proof.
+Admitted.
+
+Lemma dir2flatmem_delete_file: forall (F: @pred (list string) (@list_eq_dec string string_dec) (addr * BFILE.bfile))
+     tree name inum f basenum basedents base,
+  tree_names_distinct tree ->
+  DIRTREE.find_subtree base tree = Some (DIRTREE.TreeDir basenum basedents) ->
+  (F * (base++[name])%list |-> (inum, f))%pred (dir2flatmem [] tree) ->
+  F (dir2flatmem [] (update_subtree base (TreeDir basenum (delete_from_list name basedents)) tree)).
+Proof.
+  intros.
+  erewrite dir2flatmem_update_delete; eauto.
+  eapply ptsto_mem_except; eauto.
+  pred_apply.
+  cancel.
+Qed.
+
 
 Global Opaque dir2flatmem.
